\begin{enumerate}
    \item \[L : \left\{\begin{aligned}
        x - y - 4z + 12 = 0 \\ 2x + y - 2z + 3 = 0
    \end{aligned}\right.\qquad \Longrightarrow\qquad \left\{\begin{aligned}
        &x + 5 = 2z \\ & 7 - y = 2z
    \end{aligned}\right.\qquad\Longrightarrow\qquad \frac{x + 5}{2} = \frac{7 - y}{2} = z\]

    \item \(\forall\; M \in L\)，\(M\)可以表示成如下形式\[M(2t - 5 , 7 - 2t, t)\qquad\Longrightarrow\qquad\overrightarrow{PM} = (2t - 7, 7 - 2t, t + 1) \]
    由于直线的方向向量\(\boldsymbol{n} = (2, -2, 1)\)
    ，故由几何关系\[\overrightarrow{PM}\cdot \boldsymbol{n} = (2t - 7, 7 - 2t, t + 1)\cdot(2, -2, 1) = 0\qquad \Longrightarrow\qquad t = 3 \qquad \Longrightarrow\qquad M(1, 1, 3)\]
    其中\(M\)就是过点\(P\)在直线\(L\)上的垂足。设对称点为\(P_1(x, y, z)\)，那么\(M\)是\(PP_1\)的中点，故\[\left\{\begin{aligned}
        &2 + x = 2 \\ & y = 2 \\ &1 + z = 6
    \end{aligned}\right. \qquad\Longrightarrow\qquad \left\{\begin{aligned}
        &x = 0 \\ & y = 2 \\ & z = 5
    \end{aligned}\right.\]
    故对称点为\((0, 2, 5).\)
    
\end{enumerate}