\paragraph*{3.5-1}

令 $x=\tan t$, 有
\[
\begin{aligned}
	\int \dfrac{x^3\,\mathrm dx}{\sqrt{1+x^2}}&=\int\dfrac{\tan^3 t\sec^2 t}{\sec t}\,\mathrm dt\\
	&=\int \tan^2 t\cdot\tan t\sec t\\
	&=\int (\sec^2 t-1)\,\mathrm d\sec t\\
	&=\dfrac{1}{3}\sec^3 t-\sec t+C=\dfrac{1}{3}\left(1+x^2\right)^{\frac{3}{2}}-\left(1+x^2\right)^{\frac{1}{2}}+C 
\end{aligned}
\]
\paragraph*{3.5-2}
\[
	\begin{aligned}
\dfrac{x^3\,\mathrm dx}{\sqrt{1+x^2}}&=\dfrac{1}{2}\int\dfrac{x^2}{\sqrt{1+x^2}}\,\mathrm d\left(1+x^2\right)\\
&=\int x^2\,\mathrm d\sqrt{1+x^2}=\int\left(\sqrt{1+x^2}\right)^2\,\mathrm d\sqrt{1+x^2}-\int\,\mathrm d\sqrt{1+x^2}\\
&=\dfrac{1}{3}\left(1+x^2\right)^{\frac{3}{2}}-\left(1+x^2\right)^{\frac{1}{2}}+C 
	\end{aligned}
\]
\paragraph*{3.5-3}
\[
	\begin{aligned}
\int\dfrac{x^3\,\mathrm dx}{\sqrt{1+x^2}}&=\dfrac{1}{2}\int\dfrac{x^2}{\sqrt{1+x^2}}\,\mathrm d\left(1+x^2\right)\\
&=\dfrac{1}{2}\int\dfrac{1+x^2-1}{\sqrt{1+x^2}}\,\mathrm d\left(1+x^2\right)\\
&=\dfrac{1}{2}\int\left(\left(1+x^2\right)^{\frac{1}{2}}-\left(1+x^2\right)^{-\frac{1}{2}}\right)\,\mathrm d\left(1+x^2\right)\\
&=\dfrac{1}{3}\left(1+x^2\right)^{\frac{3}{2}}-\left(1+x^2\right)^{\frac{1}{2}}+C 
	\end{aligned}
\]